\documentclass{article}
\usepackage{amsfonts}
\usepackage{amsmath}
\begin{document}
	
% % % Page 1 % % %
\textbf{\LARGE Author: Keith Stellyes}\\

\textbf{\Large A few proofs regarding algorithms}\\

Page 2: \texttt{Bubble Sort (INCOMPLETE)}

Page 3: \texttt{Knuth Volume 1. Chapter 1. Problem 2 (Euclidean Algorithm)}

\newpage
% % % Page 2 % % %

\textbf{\Large A proof on bubble sort}\\

% ( a work in progress )

A sorted set is defined as follows (Where $S_{0}$ is the initial element): 

$$S_{k} \leq S_{k + 1} \vee$$ 
$$S_{k} = |S| - 1$$

\texttt{procedure bubbleSort(S : Ordered set)}

\qquad\texttt{swapped $\leftarrow true$}

\qquad\texttt{while swapped}

\qquad\qquad\texttt{swapped $\leftarrow false$}

\qquad\qquad\texttt{for n $\rightarrow$ |S| - 2}

\qquad\qquad\qquad\texttt{if $S_{n} >  S_{n + 1}$}

\qquad\qquad\qquad\qquad\texttt{Swap($S_{n}$, $S_{n + 1}$)}

\qquad\qquad\qquad\qquad\texttt{swapped $\leftarrow true$}

\newpage

% % % Page 3 % % %
\textbf{\Large A proof to solve a problem from Knuth regarding Euclidean Algorithm}\\

2. [15] Prove that $m$ is always greater than $n$ at the beginning of step \textbf{E1}, after it has already occurred once. Where E1 is part of the algorithm, \textbf{E}:\\

\textbf{Algorithm E:}\\

\textbf{E1}: Divide $m$ by $n$ and let $r$ be the remainder.

\textbf{E2}: If $r = 0$: return n

\textbf{E3}: $m \leftarrow n , n \leftarrow r$ goto \textbf{E1}\\

Proof:\\

Prove that $m_{k} > n_{k}$ where $k > 0$\\\

Let:\

\hspace{1cm} $m_{k} = n_{k - 1}$

\hspace{1cm} $n_{k} = m_{k - 1}$ mod $n_{k - 1}$\

\hspace{1cm} $n_{k} \neq 0$\ 

\hspace{1cm} $k = 0$ at the first time at \textbf{E1}\

\hspace{1cm} $k > 0$\\

% mk-1 > nk-1
% mk-1 < nk-1
% mk-1 = nk-1

$m_{k} > n_{k} \rightarrow$

$n_{k-1} > m_{k-1}$ mod $n_{k-1}$\\

\textbf{Case I} $m_{k - 1} = n_{k - 1}$:\

\hspace{1cm} Impossible:

\hspace{1cm} $m_{k - 1} = n_{k - 1} \rightarrow m_{k - 1}$ mod $n_{k - 1} = 0$\

\hspace{1cm} $n_{k} = m_{k - 1}$ mod $n_{k - 1} = 0 \rightarrow$\

\hspace{1cm} $n_{k} = 0 \wedge n_{k} \neq 0$ \hfill Contradiction\\

\textbf{Case II} $m_{k - 1} > n_{k - 1}$:\

\hspace{1cm} 1. $m_{k - 1} > n_{k - 1} \rightarrow$\

\hspace{1cm} 2. $n_{k-1} > m_{k - 1}$ mod $n_{k - 1}$\

\hspace{1cm} 3. $m_{k} > n_{k}$\\


\textbf{Case III} $m_{k - 1} < n_{k - 1}$:\

\hspace{1cm} 1. $m_{k - 1} < n_{k - 1} \rightarrow$\

\hspace{1cm} 2. $m_{k - 1}$ mod $n_{k - 1} = m_{k - 1} \rightarrow$\

\hspace{1cm} 3. $m_{k} = n_{k - 1}> m_{k - 1} \wedge$\ \hfill Definition of case

\hspace{1cm} 4. $n_{k} = m_{k - 1}$ \hfill 2

\hspace{1cm} 5. $m_{k} > n_{k}$

\end{document}