\documentclass{article}
\usepackage{amsfonts}
\usepackage{amsmath}
\begin{document}
	
\textbf{Author: Keith Stellyes}\\

Proof that \texttt{k << 1 = k * 2} where \texttt{<<} is the bitshift left operation and k is an integer represented as a series of bits.\

The bit string ordered set $B$ is equal to the integer $I(B)$ where:

$$I(B) = \sum_{k=0}^{|B| - 1} 2^{k} \times B_{k}$$

For convenience, we define a function, $bi(b, k)$ where $b = 0 \oplus b = 1$ where:

$$bi(b, k) = 2^{k} \times b$$

Which lets us re-express $I(B)$ as:

$$I(B) = \sum_{k=0}^{|B| - 1} bi(B_{k}, k)$$

The bit string representing the left bitshift is defined by the function $lshift(B)$ where:

$$lshift(B)_{k} = \begin{cases}
0 & \mbox{if } k \leq 0\\
B_{k - 1} & \mbox{if } k > 0
\end{cases}
$$

We want to prove the following: $$I(lshift(B)) = 2 \times I(B) = $$ 

$$\sum_{k=0}^{|B| - 1} bi(B_{k}, k) = 2 \times \sum_{k=0}^{|B| - 1} bi(lshift(B)_{k}, k)$$

For $k > 0$

$$bi(m, n + 1) = 2 \times bi(m, n)$$

$$2 \times 2^{n} \times m = 2^{n + 1} \times m$$

$k+1$ to maintain the magnitude...:

$$bi(lshift(B)_{k}, k) = bi({B_{k - 1}, k + 1}) = 2 \times bi(B_{k - 1}, k)$$

Finally...

$$\sum_{k=0}^{|B| - 1} bi(B_{k}, k) = 2 \times \sum_{k=0}^{|B| - 1} bi(B_{k - 1}, k) = $$

$$2 \times \sum_{k=0}^{|B| - 1} bi(leftshift(B_{k}), k)$$

\end{document}